examples/gen_conn/proofs.v
@@ -87,7 +87,7 @@ Lemma wp_listen c N ps :
       public ga ∗ minted skI }}}.
 Proof.
 iIntros "#? #? [[#? _] _] % !> _ post". wp_lam.
-wp_apply wp_responder_wait; eauto.
+wp_apply wp_responder_listen; eauto.
 Qed.
 
 Lemma wp_confirm P ps c skI skR ga N :
@@ -121,7 +121,7 @@ wp_bind (do_until _).
 iApply (wp_frame_wand with "post").
 iApply (wp_frame_wand with "P").
 iApply wp_do_until'. iIntros "!>".
-wp_pures. iApply (wp_responder_accept failed).
+wp_pures. iApply (wp_responder_confirm failed).
 { do !iSplit => //=.
   iIntros "%gb token".
   rewrite (term_token_difference _ (↑iso_dhN.@"res".@"chan"));
